Simplifications

Typed_Arithmetic_Expressions.thy
@@ -6,212 +6,119 @@ begin
 
 chapter {* Typed Arithmetic Expressions *}
 
-datatype_new NBTerm
-  = NBTrue
-  | NBFalse
-  | NBIf NBTerm NBTerm NBTerm
-  | NBZero
-  | NBSucc NBTerm
-  | NBPred NBTerm
-  | NBIs_zero NBTerm
+datatype NBTerm =
+  NBTrue
+| NBFalse
+| NBIf NBTerm NBTerm NBTerm
+| NBZero
+| NBSucc NBTerm
+| NBPred NBTerm
+| NBIs_zero NBTerm
 
 section {* Types *}
 
-datatype_new Type
-  = Bool
-  | Nat
+text {* The language of arithmetic expressions contains two types of expressions: booleans and
+natural numbers.*}
+
+datatype Type = Bool | Nat
 
 section {* The Typing Relation *}
 
 text {* Definition 8.2.1 *}
 
-inductive has_type :: "NBTerm \<Rightarrow> Type \<Rightarrow> bool" where
-  has_type_NBTrue: "has_type NBTrue Bool" |
-  has_type_NBFalse: "has_type NBFalse Bool" |
-  has_type_NBIf: "has_type t1 Bool \<Longrightarrow> has_type t2 T \<Longrightarrow> has_type t3 T \<Longrightarrow> has_type (NBIf t1 t2 t3) T" |
-  has_type_NBZero: "has_type NBZero Nat" |
-  has_type_NBSucc: "has_type t Nat \<Longrightarrow> has_type (NBSucc t) Nat" |
-  has_type_NBPred: "has_type t Nat \<Longrightarrow> has_type (NBPred t) Nat" |
-  has_type_NBIs_zero: "has_type t Nat \<Longrightarrow> has_type (NBIs_zero t) Bool"
+inductive has_type :: "NBTerm \<Rightarrow> Type \<Rightarrow> bool" (infix "|:|" 150) where
+  has_type_NBTrue: "NBTrue |:| Bool" |
+  has_type_NBFalse: "NBFalse |:| Bool" |
+  has_type_NBIf: "t1 |:| Bool \<Longrightarrow> t2 |:| T \<Longrightarrow> t3 |:| T \<Longrightarrow> NBIf t1 t2 t3 |:| T" |
+  has_type_NBZero: "NBZero |:| Nat" |
+  has_type_NBSucc: "t |:| Nat \<Longrightarrow> NBSucc t |:| Nat" |
+  has_type_NBPred: "t |:| Nat \<Longrightarrow> NBPred t |:| Nat" |
+  has_type_NBIs_zero: "t |:| Nat \<Longrightarrow> NBIs_zero t |:| Bool"
 
 text {* Lemma 8.2.2 *}
 
 lemma inversion_of_typing_relation:
-  "has_type NBTrue R \<Longrightarrow> R = Bool"
-  "has_type NBFalse R \<Longrightarrow> R = Bool"
-  "has_type (NBIf t1 t2 t3) R \<Longrightarrow> has_type t1 Bool \<and> has_type t2 R \<and> has_type t3 R"
-  "has_type NBZero R \<Longrightarrow> R = Nat"
-  "has_type (NBSucc t) R \<Longrightarrow> R = Nat \<and> has_type t Nat"
-  "has_type (NBPred t) R \<Longrightarrow> R = Nat \<and> has_type t Nat"
-  "has_type (NBIs_zero t) R \<Longrightarrow> R = Bool \<and> has_type t Nat"
+  "NBTrue |:| R \<Longrightarrow> R = Bool"
+  "NBFalse |:| R \<Longrightarrow> R = Bool"
+  "NBIf t1 t2 t3 |:| R \<Longrightarrow> t1 |:| Bool \<and> t2 |:| R \<and> t3 |:| R"
+  "NBZero |:| R \<Longrightarrow> R = Nat"
+  "NBSucc t |:| R \<Longrightarrow> R = Nat \<and> t |:| Nat"
+  "NBPred t |:| R \<Longrightarrow> R = Nat \<and> t |:| Nat"
+  "NBIs_zero t |:| R \<Longrightarrow> R = Bool \<and> t |:| Nat"
   by (auto elim: has_type.cases)
 
 text {* Theorem 8.2.4 *}
 
 theorem has_type_right_unique:
-  "has_type t T \<Longrightarrow> has_type t T' \<Longrightarrow> T = T'"
-proof (induction t T arbitrary: T' rule: has_type.induct)
-  case has_type_NBTrue
-  thus ?case by (metis inversion_of_typing_relation(1))
-next
-  case has_type_NBFalse
-  thus ?case by (metis inversion_of_typing_relation(2))
-next
-  case (has_type_NBIf t1 t2 T t4)
-  thus ?case by (metis inversion_of_typing_relation(3))
-next
-  case has_type_NBZero
-  thus ?case by (metis inversion_of_typing_relation(4))
-next
-  case has_type_NBSucc
-  thus ?case by (metis inversion_of_typing_relation(5))
-next
-  case has_type_NBPred
-  thus ?case by (metis inversion_of_typing_relation(6))
-next
-  case has_type_NBIs_zero
-  thus ?case by (metis inversion_of_typing_relation(7))
-qed
+  "t |:| T \<Longrightarrow> t |:| T' \<Longrightarrow> T = T'"
+by (induction t T rule: has_type.induct) (auto dest: inversion_of_typing_relation)
 
 section {* Safety = Progress + Preservation *}
 
 inductive is_numeric_value :: "NBTerm \<Rightarrow> bool" where
-  is_numeric_value_NBZero: "is_numeric_value NBZero" |
-  is_numeric_value_NBSucc: "is_numeric_value nv \<Longrightarrow> is_numeric_value (NBSucc nv)"
+  "is_numeric_value NBZero" |
+  "is_numeric_value nv \<Longrightarrow> is_numeric_value (NBSucc nv)"
 
 inductive is_value :: "NBTerm \<Rightarrow> bool" where
-  is_value_NBTrue: "is_value NBTrue" |
-  is_value_NBFalse: "is_value NBFalse" |
-  is_value_numeric_value: "is_numeric_value nv \<Longrightarrow> is_value nv"
+  "is_value NBTrue" |
+  "is_value NBFalse" |
+  "is_numeric_value nv \<Longrightarrow> is_value nv"
 
 text {* Lemma 8.3.1 *}
 
 lemma canonical_form:
-  "is_value v \<Longrightarrow> has_type v Bool \<Longrightarrow> v = NBTrue \<or> v = NBFalse"
-  "is_value v \<Longrightarrow> has_type v Nat \<Longrightarrow> is_numeric_value v"
+  "is_value v \<Longrightarrow> v |:| Bool \<Longrightarrow> v = NBTrue \<or> v = NBFalse"
+  "is_value v \<Longrightarrow> v |:| Nat \<Longrightarrow> is_numeric_value v"
   by (auto elim: has_type.cases is_value.cases is_numeric_value.cases)
 
 inductive eval_once :: "NBTerm \<Rightarrow> NBTerm \<Rightarrow> bool" where
-  eval_once_NBIf_NBTrue: "eval_once (NBIf NBTrue t2 t3) t2" |
-  eval_once_NBIf_NBFalse: "eval_once (NBIf NBFalse t2 t3) t3" |
-  eval_once_NBIf: "eval_once t1 t1' \<Longrightarrow> eval_once (NBIf t1 t2 t3) (NBIf t1' t2 t3)" |
-  eval_once_NBSucc: "eval_once t1 t1' \<Longrightarrow> eval_once (NBSucc t1) (NBSucc t1')" |
-  eval_once_NBPred_NBZero: "eval_once (NBPred NBZero) NBZero" |
-  eval_once_NBPred_NBSucc: "is_numeric_value nv1 \<Longrightarrow> eval_once (NBPred (NBSucc nv1)) nv1" |
-  eval_once_NBPred: "eval_once t1 t1' \<Longrightarrow> eval_once (NBPred t1) (NBPred t1')" |
-  eval_once_NBIs_zero_NBZero: "eval_once (NBIs_zero NBZero) NBTrue" |
-  eval_once_NBIs_zero_NBSucc: "is_numeric_value nv1 \<Longrightarrow> eval_once (NBIs_zero (NBSucc nv1)) NBFalse" |
-  eval_once_NBIs_zero: "eval_once t1 t1' \<Longrightarrow> eval_once (NBIs_zero t1) (NBIs_zero t1')"
+  "eval_once (NBIf NBTrue t2 t3) t2" |
+  "eval_once (NBIf NBFalse t2 t3) t3" |
+  "eval_once t1 t1' \<Longrightarrow> eval_once (NBIf t1 t2 t3) (NBIf t1' t2 t3)" |
+  "eval_once t1 t1' \<Longrightarrow> eval_once (NBSucc t1) (NBSucc t1')" |
+  "eval_once (NBPred NBZero) NBZero" |
+  "is_numeric_value nv1 \<Longrightarrow> eval_once (NBPred (NBSucc nv1)) nv1" |
+  "eval_once t1 t1' \<Longrightarrow> eval_once (NBPred t1) (NBPred t1')" |
+  "eval_once (NBIs_zero NBZero) NBTrue" |
+  "is_numeric_value nv1 \<Longrightarrow> eval_once (NBIs_zero (NBSucc nv1)) NBFalse" |
+  "eval_once t1 t1' \<Longrightarrow> eval_once (NBIs_zero t1) (NBIs_zero t1')"
 
 text {* Theorem 8.3.2 *}
 
-theorem progress: "has_type t T \<Longrightarrow> is_value t \<or> (\<exists>t'. eval_once t t')"
+theorem progress: "t |:| T \<Longrightarrow> is_value t \<or> (\<exists>t'. eval_once t t')"
 proof (induction t T rule: has_type.induct)
   case has_type_NBTrue
-  thus ?case by (auto intro: is_value_NBTrue)
+  thus ?case by (auto intro: is_value.intros)
 next
   case has_type_NBFalse
-  thus ?case by (auto intro: is_value_NBFalse)
+  thus ?case by (auto intro: is_value.intros)
 next
   case (has_type_NBIf t1 t2 T t3)
-  have "\<exists>t'. eval_once (NBIf t1 t2 t3) t'"
-    proof (cases "is_value t1")
-      case True
-      thus "\<exists>t'. eval_once (NBIf t1 t2 t3) t'"
-        by (auto
-          intro: has_type_NBIf.hyps(1) eval_once_NBIf_NBTrue eval_once_NBIf_NBFalse
-          dest: canonical_form)
-    next
-      case False
-      thus "\<exists>t'. eval_once (NBIf t1 t2 t3) t'"
-        using has_type_NBIf.IH(1)
-        by (auto intro: eval_once_NBIf)
-    qed
-  thus ?case by simp
+  thus ?case by (cases "is_value t1") (auto intro: eval_once.intros dest: canonical_form)
 next
   case has_type_NBZero
-  thus ?case  by (auto intro: is_value_numeric_value is_numeric_value_NBZero)
+  thus ?case  by (auto intro: is_value.intros is_numeric_value.intros)
 next
   case (has_type_NBSucc t)
-  show "?case"
-    proof (cases "is_value t")
-      case True
-      thus "is_value (NBSucc t) \<or> (\<exists>a. eval_once (NBSucc t) a)"
-        by (auto
-          intro: is_value_numeric_value is_numeric_value_NBSucc
-          dest!: canonical_form
-          simp: has_type_NBSucc.hyps)
-    next
-      case False
-      thus "is_value (NBSucc t) \<or> (\<exists>a. eval_once (NBSucc t) a)"
-        by (metis eval_once_NBSucc has_type_NBSucc.IH)
-    qed
+  thus ?case by (cases "is_value t")
+    (auto intro: eval_once.intros is_value.intros is_numeric_value.intros dest: canonical_form)
 next
   case (has_type_NBPred t)
-  show ?case
-    proof (cases "is_value t")
-      case True
-      thus "is_value (NBPred t) \<or> (\<exists>a. eval_once (NBPred t) a)"
-        by (auto
-          intro: eval_once_NBPred_NBZero eval_once_NBPred_NBSucc is_numeric_value.cases
-          dest!: canonical_form
-          simp: has_type_NBPred.hyps)
-    next
-      case False
-      thus "is_value (NBPred t) \<or> (\<exists>a. eval_once (NBPred t) a)"
-        by (metis eval_once_NBPred has_type_NBPred.IH)
-    qed
+  thus ?case by (cases "is_value t")
+    (auto intro: eval_once.intros is_numeric_value.cases dest: canonical_form)
 next
   case (has_type_NBIs_zero t)
-  show ?case
-    proof (cases "is_value t")
-      case True
-      thus "is_value (NBIs_zero t) \<or> (\<exists>a. eval_once (NBIs_zero t) a)"
-        by (auto
-          intro: eval_once_NBIs_zero_NBZero eval_once_NBIs_zero_NBSucc is_numeric_value.cases
-          dest!: canonical_form
-          simp: has_type_NBIs_zero.hyps)
-    next
-      case False
-      thus "is_value (NBIs_zero t) \<or> (\<exists>a. eval_once (NBIs_zero t) a)"
-        using has_type_NBIs_zero.IH
-        by (auto intro: eval_once_NBIs_zero)
-    qed
+  thus ?case by (cases "is_value t")
+    (auto intro: eval_once.intros is_numeric_value.cases dest: canonical_form)
 qed
 
 text {* Theorem 8.3.3 *}
 
-inductive_cases eval_once_NBTrueE: "eval_once NBTrue t"
-inductive_cases eval_once_NBFalseE: "eval_once NBFalse t"
-inductive_cases eval_once_NBZeroE: "eval_once NBZero t"
-inductive_cases eval_once_NBSuccE: "eval_once (NBSucc t) t'"
-inductive_cases eval_once_NBPredE: "eval_once (NBPred t) t'"
-inductive_cases eval_once_NBIs_zeroE: "eval_once (NBIs_zero t) t'"
-
-theorem preservation: "has_type t T \<Longrightarrow> eval_once t t' \<Longrightarrow> has_type t' T"
+theorem preservation: "t |:| T \<Longrightarrow> eval_once t t' \<Longrightarrow> t' |:| T"
 proof (induction t T arbitrary: t' rule: has_type.induct)
-  case has_type_NBTrue
-  thus ?case by (rule eval_once_NBTrueE)
-next
-  case has_type_NBFalse
-  thus ?case by (rule eval_once_NBFalseE)
-next
   case (has_type_NBIf t1 t2 T t3)
   from has_type_NBIf.prems has_type_NBIf.IH has_type_NBIf.hyps show ?case
-    by (cases rule: eval_once.cases) (auto intro: has_type.has_type_NBIf)
-next
-  case has_type_NBZero
-  thus ?case by (rule eval_once_NBZeroE)
-next
-  case (has_type_NBSucc t)
-  thus ?case by (auto intro: has_type.intros elim: eval_once_NBSuccE)
-next
-  case (has_type_NBPred t)
-  thus ?case
-    by (auto intro: has_type.intros dest: inversion_of_typing_relation elim: eval_once_NBPredE)
-next
-  case (has_type_NBIs_zero t)
-  thus ?case by (auto intro: has_type.intros elim: eval_once_NBIs_zeroE)
-qed
+    by (auto intro: has_type.has_type_NBIf elim: eval_once.cases)
+qed (auto intro: has_type.intros dest: inversion_of_typing_relation elim: eval_once.cases)
 
 end
